theories/lex_list.v
@@ -1,0 +1,377 @@
+(**************************************************************)
+(*   Copyright Dominique Larchey-Wendling [*]                 *)
+(*                                                            *)
+(*                             [*] Affiliation LORIA -- CNRS  *)
+(**************************************************************)
+(*      This file is distributed under the terms of the       *)
+(*        Mozilla Public License Version 2.0, MPL-2.0         *)
+(**************************************************************)
+
+From Coq Require Import List Relations Wellfounded Utf8.
+From Hydra Require Import hydra ordered.
+
+Import ListNotations.
+
+Set Implicit Arguments.
+
+#[local] Infix "∈" := In (at level 70, no associativity).
+#[local] Arguments clos_trans {_}.
+#[local] Arguments clos_refl_trans {_}.
+#[local] Arguments transitive {_}.
+
+#[local] Hint Constructors clos_trans clos_refl_trans : core.
+#[local] Hint Resolve Acc_inv Acc_intro in_cons in_eq in_elt in_or_app : core.
+
+Section clos_trans.
+
+  Variables (X : Type).
+
+  Implicit Type (R T : X → X → Prop).
+
+  Hint Constructors clos_refl_trans : core.
+
+  Fact clos_t_rt R x y z :
+       clos_trans R x y → clos_refl_trans R y z → clos_trans R x z.
+  Proof. induction 2; eauto. Qed.
+
+  Fact clos_trans_ge R : transitive R → ∀ x y, clos_trans (ge R) x y → ge R x y.
+  Proof. 
+    intros HR; red in HR.
+    induction 1 as [ ? ? [] | ? ? ? _ [] _ [] ]; subst; eauto.
+  Qed.
+
+  Fact clos_t_ge_rt R x y : clos_trans (ge R) x y → clos_refl_trans R y x.
+  Proof. induction 1 as [ ? ? [ <- | ] | ]; eauto. Qed.
+
+  Fact clos_trans_mono R T : 
+          (∀ x y, R x y → T x y)
+        → (∀ l m, clos_trans R l m → clos_trans T l m).
+  Proof. induction 2; eauto. Qed.
+
+End clos_trans.
+
+Fact list_snoc_rect {X} (P : list X → Type) :
+           P []
+         → (∀ l x, P l → P (l++[x]))
+         → ∀ l, P l.
+Proof.
+  intros H1 H2 l; revert P H1 H2.
+  induction l as [ | x l IHl ]; auto.
+  intros P H1 H2.
+  apply (IHl (fun l => P (x::l))).
+  + apply (H2 []), H1.
+  + intros ? ?; apply (H2 (_::_)).
+Qed.
+
+Inductive list_snoc_inv_t X : list X → Type :=
+  | in_list_snoc_inv_t l x : list_snoc_inv_t (l++[x]).
+
+Fact list_snoc_inv X (l : list X) : l ≠ [] → list_snoc_inv_t l.
+Proof.
+  destruct l as [ | l x ] using list_snoc_rect.
+  + now intros [].
+  + intros; constructor.
+Qed.
+
+Section lex_list.
+
+  Variables (X : Type) (R : X → X → Prop).
+
+  (* lexicographic order on lists, head is most significant *)
+  Inductive lex_list : list X → list X → Prop :=
+    | lex_list_nil x m : lex_list [] (x::m)
+    | lex_list_lt x y l m : R x y → lex_list (x::l) (y::m)
+    | lex_list_eq x l m : lex_list l m → lex_list (x::l) (x::m).
+
+  Hint Constructors lex_list : core.
+
+  Inductive lex_list_inv_t l m : X → X → Prop :=
+    | in_lex_list_inv_t0 x y : R x y → lex_list_inv_t l m x y
+    | in_lex_list_inv_t1 x : lex_list l m → lex_list_inv_t l m x x.
+
+  Hint Constructors lex_list_inv_t : core.
+
+  Fact lex_list_inv l m :
+         lex_list l m 
+       ↔ match l, m with 
+         | _, []      => False
+         | [], _      => True
+         | x::l, y::m => lex_list_inv_t l m x y
+         end.
+  Proof. 
+    split.
+    + intros []; eauto.
+    + revert l m; intros [] [] []; eauto.
+  Qed.
+
+  Inductive lex_list_invert_t : list X → list X → Prop :=
+    | in_lex_list_invert_t0 k l : k ≠ [] → lex_list_invert_t l (l++k)
+    | in_lex_list_invert_t1 p x y l m : R x y → lex_list_invert_t (p++[x]++l) (p++[y]++m).
+
+  Hint Constructors lex_list_invert_t : core.
+
+  Lemma lex_list_invert l m : lex_list l m → lex_list_invert_t l m.
+  Proof.
+    induction 1 as [ x m | x y l m H | z l m _ [] ].
+    + now constructor 1 with (l := []).
+    + now constructor 2 with (p := []).
+    + now constructor 1 with (l := _::_).
+    + now constructor 2 with (p := _::_).
+  Qed.
+
+  Inductive lex_list_snoc_inv_t y : list X → list X → Prop :=
+    | in_lex_list_snoc_inv_t0 l m : lex_list_snoc_inv_t y l (l++m)
+    | in_lex_list_snoc_inv_t1 x l m : R x y → lex_list_snoc_inv_t y (l++[x]++m) l
+    | in_lex_list_snoc_inv_t2 p u v l m : R u v → lex_list_snoc_inv_t y (p++[u]++l) (p++[v]++m).
+
+  Local Lemma lex_list_snoc_inv_rec l m' : lex_list l m' → ∀ m y, m' = m++[y] → lex_list_snoc_inv_t y l m.
+  Proof.
+    intros [ ? m [k x]%list_snoc_inv | ]%lex_list_invert.
+    + intros ? ?; rewrite <- app_ass; intros [ <- <- ]%app_inj_tail; constructor.
+    + destruct m as [ | m z _ ] using list_snoc_rect.
+      * intros ? ?; rewrite <- app_nil_end; intros [ <- <- ]%app_inj_tail; now constructor.
+      * intros ? ?; rewrite <- !app_ass; intros [ <- <- ]%app_inj_tail; rewrite !app_ass; now constructor.
+  Qed.
+
+  Lemma lex_list_snoc_inv l y m : lex_list l (m++[y]) → lex_list_snoc_inv_t y l m.
+  Proof. intros; eapply lex_list_snoc_inv_rec; eauto. Qed.
+
+  Inductive lex_list_sg_inv_right_t y : list X → Prop :=
+    | in_lex_list_sg_inv_right_t0 : lex_list_sg_inv_right_t y []
+    | in_lex_list_sg_inv_right_t1 x l : R x y → lex_list_sg_inv_right_t y (x::l).
+
+  Lemma lex_list_sg_inv_right l y : lex_list l [y] → lex_list_sg_inv_right_t y l.
+  Proof.
+    revert l; intros [ | x l ].
+    + intros []%lex_list_inv; constructor.
+    + intros [ | ? ?%lex_list_inv ]%lex_list_inv; constructor; auto.
+      now destruct l.
+  Qed.
+
+  Fact lex_list_app_head c l m : lex_list l m → lex_list (c++l) (c++m).
+  Proof. induction c; simpl; eauto. Qed.
+
+  Fact lex_list_prefix p l : l <> [] → lex_list p (p++l).
+  Proof. 
+    destruct l; [ easy | intros _ ].
+    rewrite (app_nil_end p) at 1.
+    apply lex_list_app_head; auto.
+  Qed.
+
+  Fact lex_list_snoc h l : lex_list l (l++[h]).
+  Proof. now apply lex_list_prefix. Qed.
+
+  Hint Constructors sdec : core.
+
+  Section lex_list_total.
+
+    Variables (l m : list X)
+              (Hlm : ∀ x y, x ∈ l → y ∈ m → sdec R x y).
+
+    Theorem lex_list_sdec : sdec lex_list l m.
+    Proof.
+      revert m Hlm.
+      rename l into l'.
+      induction l' as [ | x l IHl ]; intros [ | y m ] Hlm; eauto.
+      destruct (Hlm x y) as [ x y H | x | x y H ]; eauto.
+      destruct (IHl m); eauto.
+    Qed.
+
+  End lex_list_total.
+
+  Section lex_list_irrefl.
+
+    Let ll_irrefl_rec l m : lex_list l m → l = m → ∃x, x ∈ l ∧ R x x.
+    Proof.
+      induction 1 as [ | | x l m H IH ]; try easy.
+      * inversion 1; subst; eauto.
+      * injection 1; intros (? & ? & ?)%IH; eauto.
+    Qed.
+
+    Lemma lex_list_irrefl l : lex_list l l → ∃x, x ∈ l ∧ R x x.
+    Proof. intros ?%ll_irrefl_rec; auto. Qed.
+
+  End lex_list_irrefl.
+
+  Section lex_list_trans.
+
+    Variables (l m k : list X)
+              (Hlmk : ∀ x y z, x ∈ l → y ∈ m → z ∈ k → R x y → R y z → R x z).
+
+    Lemma lex_list_trans : lex_list l m → lex_list m k → lex_list l k.
+    Proof.
+      intros H1 H2; revert H1 k H2 Hlmk.
+      induction 1 as [ y m | x y l m H1 | x l m H1 IH1 ];
+        intros [] Hk%lex_list_inv; destruct Hk; eauto.
+      constructor 3; apply IH1; eauto.
+    Qed.
+
+  End lex_list_trans.
+
+End lex_list.
+
+Fact Acc_lex_list_nil X P (R : X → X → Prop) : Acc (λ l m, P l ∧ lex_list R l m) [].
+Proof. constructor; intros [] (? & []%lex_list_inv). Qed.
+
+#[local] Hint Resolve Acc_lex_list_nil : core.
+
+Section lex_list_sim.
+
+  Variables (X Y : Type) (R : X → X → Prop) (T : Y → Y → Prop)
+            (sim : X → Y → Prop)
+            (sim_fun : ∀ x y y', sim x y → sim x y' → y = y')
+            (Hsim : ∀ x y x' y', sim x y → sim x' y' → R x x' → T y y').
+
+  Hint Constructors lex_list : core.
+
+  Theorem lex_list_sim l l' m m' :
+            Forall2 sim l m
+          → Forall2 sim l' m'
+          → lex_list R l l'
+          → lex_list T m m'.
+  Proof.
+    intros H1 H2 H3; revert H3 m m' H1 H2.
+    induction 1 as [ x l' | x x' l l' | x l l' ];
+      do 2 inversion 1; subst; eauto.
+    match goal with |- lex_list _ (?a::_) (?b::_) => assert (a=b) as ->; eauto end.
+  Qed.
+
+End lex_list_sim. 
+
+Section lex_list_wf.
+
+  Variables (X : Type) (R : X → X → Prop).
+
+  Implicit Type (x : X).
+
+  Hint Constructors ordered_from clos_refl_trans : core.
+
+  Hint Resolve ordered_from_clos_trans
+               clos_t_ge_rt clos_rt_t 
+               ordered_cons_inv : core.
+
+  Fact ordered_lex_list_lo l m : ordered (ge R) l → lex_list R l m → lo (clos_trans R) l m.
+  Proof.
+    intros H1 H2; revert H2 H1.
+    induction 1 as [ x m | x y l m H1 | x l m H1 IH1 ]; intros H.
+    + apply lo_app_tail with (l := [_]), lo_intro; now simpl.
+    + apply lo_app_tail with (l := [_]), lo_intro.
+      apply ordered_inv in H.
+      intros ? [ <- | ]; eauto.
+    + apply lo_cons; eauto.
+  Qed.
+
+  Hint Resolve ordered_lex_list_lo : core.
+
+  Fact ordered_lex_list_lo_restr P l m : Forall P l → ordered (ge R) l → lex_list R l m → lo (λ x y, P x ∧ clos_trans R x y) l m.
+  Proof.
+    intros H0 H1 H2; revert H2 H1 H0.
+    induction 1 as [ x m | x y l m H1 | x l m H1 IH1 ]; intros H2 H3.
+    + apply lo_app_tail with (l := [_]), lo_intro; now simpl.
+    + apply lo_app_tail with (l := [_]), lo_intro.
+      apply ordered_inv in H2.
+      apply Forall_cons_iff in H3 as [ H3 H4 ].
+      rewrite Forall_forall in H4.
+      intros ? [ <- | ]; split; eauto.
+    + apply Forall_cons_iff in H3 as [].
+      apply lo_cons; eauto.
+  Qed.
+
+  Hint Resolve ordered_from_ge_Acc : core.
+
+  (* The proof of this lemma uses Acc for lo & the inclusion ordered_lex_list_lo 
+     CAN WE PROVIDE A MORE DIRECT PROOF *)
+  Lemma lex_list_Acc_ordered_from x l : Acc R x → ordered_from (ge R) x l → Acc (λ l m, ordered (ge R) l ∧ lex_list R l m) l.
+  Proof. 
+    intros H1 H2.
+    cut (Acc (lo (clos_trans R)) l).
+    + apply Acc_incl.
+      intros ? ? []; auto.
+    + apply Acc_lo_iff.
+      intros y Hy.
+      apply Acc_clos_trans; eauto.
+  Qed.
+
+  Hint Resolve ordered_lex_list_lo_restr : core.
+
+  (*
+
+  Lemma lex_list_Acc_ordered_from_restr P x l :
+             Acc (λ x y, P x ∧ R x y) x
+           → Forall P l
+           → ordered_from (ge R) x l
+           → Acc (λ l m, (Forall P l ∧ ordered (ge R) l) ∧ lex_list R l m) l.
+  Proof.
+    intros H1 H2 H3.
+    cut (Acc (lo (λ x y, P x ∧ clos_trans R x y)) l).
+    + apply Acc_incl.
+      intros ? ? [[]]; eauto.
+    + apply Acc_lo_iff.
+      intros z Hz.
+      cut (Acc (clos_trans (λ x y, P x ∧ R x y)) z).
+      * apply Acc_incl.
+ admit.
+      * apply Acc_clos_trans.
+        revert H1 z Hz. 
+        apply ordered_from_ge_Acc.
+        revert H3 H2.
+        induction 1 as [ x | x y l H1 H2 IH2 ]; auto.
+        intros []%Forall_cons_iff; constructor; eauto; tauto.
+  Admitted.
+
+  *)
+
+  Theorem lex_list_Acc_ordered l : Forall (Acc R) l → ordered (ge R) l → Acc (λ l m, ordered (ge R) l ∧ lex_list R l m) l.
+  Proof.
+    intros H1 H2; revert H2 H1.
+    induction 1 as [ | x l H1 ]; intros H2; auto.
+    apply lex_list_Acc_ordered_from with x; eauto.
+    eapply Forall_forall; eauto.
+  Qed.
+ 
+  (*
+
+  Theorem lex_list_Acc_ordered_restr P l :
+           Forall P l 
+         → Forall (Acc (λ x y, P x ∧ R x y)) l 
+         → ordered (ge R) l 
+         → Acc (λ l m, (Forall P l ∧ ordered (ge R) l) ∧ lex_list R l m) l.
+  Proof.
+    intros H0 H1 H2; revert H2 H1 H0.
+    induction 1 as [ | x l H1 ]; intros H2 H3; auto.
+    apply lex_list_Acc_ordered_from_restr with x; eauto.
+    eapply Forall_forall; eauto.
+  Qed.
+
+  *)
+
+End lex_list_wf.
+
+Section mono.
+
+  Hint Constructors lex_list : core.
+
+  Variables (X : Type) (R T : X → X → Prop).
+
+  Fact lex_list_mono l m : 
+          (∀ x y, x ∈ l → y ∈ m → R x y → T x y)
+        → lex_list R l m → lex_list T l m.
+  Proof.
+    intros H.
+    induction 1 as [ | | x l m H1 IH1 ]; eauto.
+    constructor 3; eauto.
+  Qed.
+
+  Fact lo_step_mono :
+          (∀ x y, R x y → T x y)
+        → (∀ l m, lo_step R l m → lo_step T l m).
+  Proof. induction 2; constructor; eauto. Qed.
+
+  Hint Resolve lo_step_mono : core.
+
+  Fact lo_mono :
+          (∀ x y, R x y → T x y)
+        → (∀ l m, lo R l m → lo T l m).
+  Proof. intro; apply clos_trans_mono; eauto. Qed.
+
+End mono.
